Expand the endian-ness library with conversions, operators for indexing arrays with proper commutations between seq_uint32_of_le and S.index

kremlib/FStar.Kremlin.Endianness.fst
@@ -1,29 +1,29 @@
 module FStar.Kremlin.Endianness
 
-open FStar.Seq
 open FStar.Mul
 open FStar.HyperStack.All
 
 module U8 = FStar.UInt8
 module U32 = FStar.UInt32
 module Math = FStar.Math.Lemmas
+module S = FStar.Seq
 
 (* Selectively imported from Hacl*'s FStar.Endianness.fst library, with several
 name changes *)
 
-type bytes = seq U8.t
+type bytes = S.seq U8.t
 
 /// lt_to_n interprets a byte sequence as a little-endian natural number
-val le_to_n : b:bytes -> Tot nat (decreases (length b))
+val le_to_n : b:bytes -> Tot nat (decreases (S.length b))
 let rec le_to_n b =
-  if Seq.length b = 0 then 0
-  else U8.v (head b) + pow2 8 * le_to_n (tail b)
+  if S.length b = 0 then 0
+  else U8.v (S.head b) + pow2 8 * le_to_n (S.tail b)
 
 /// be_to_n interprets a byte sequence as a big-endian natural number
-val be_to_n : b:bytes -> Tot nat (decreases (length b))
+val be_to_n : b:bytes -> Tot nat (decreases (S.length b))
 let rec be_to_n b =
-  if Seq.length b = 0 then 0
-  else U8.v (last b) + pow2 8 * be_to_n (slice b 0 (length b - 1))
+  if S.length b = 0 then 0
+  else U8.v (S.last b) + pow2 8 * be_to_n (S.slice b 0 (S.length b - 1))
 
 private val lemma_euclidean_division: r:nat -> b:nat -> q:pos -> Lemma
   (requires (r < q))
@@ -78,11 +78,11 @@ let rec lemma_be_to_n_is_bounded b =
 /// n_to_le encodes a number as a little-endian byte sequence of a fixed,
 /// sufficiently large length
 val n_to_le : len:U32.t -> n:nat{n < pow2 (8 * U32.v len)} ->
-  Tot (b:bytes{length b == U32.v len /\ n == le_to_n b})
+  Tot (b:bytes{S.length b == U32.v len /\ n == le_to_n b})
   (decreases (U32.v len))
 let rec n_to_le len n =
   if len = 0ul then
-    empty
+    S.empty
   else
     let len = U32.(len -^ 1ul) in
     let byte = U8.uint_to_t (n % 256) in
@@ -90,19 +90,19 @@ let rec n_to_le len n =
     Math.pow2_plus 8 (8 * U32.v len);
     assert(n' < pow2 (8 * U32.v len ));
     let b' = n_to_le len n' in
-    let b = cons byte b' in
-    lemma_eq_intro b' (tail b);
+    let b = S.cons byte b' in
+    S.lemma_eq_intro b' (S.tail b);
     b
 
 /// n_to_be encodes a numbers as a big-endian byte sequence of a fixed,
 /// sufficiently large length
 val n_to_be:
   len:U32.t -> n:nat{n < pow2 (8 * U32.v len)} ->
-  Tot (b:bytes{length b == U32.v len /\ n == be_to_n b})
+  Tot (b:bytes{S.length b == U32.v len /\ n == be_to_n b})
   (decreases (U32.v len))
 let rec n_to_be len n =
   if len = 0ul then
-    empty
+    S.empty
   else
     let len = U32.(len -^ 1ul) in
     let byte = U8.uint_to_t (n % 256) in
@@ -110,9 +110,9 @@ let rec n_to_be len n =
     Math.pow2_plus 8 (8 * U32.v len);
     assert(n' < pow2 (8 * U32.v len ));
     let b' = n_to_be len n' in
-    let b'' = create 1 byte in
-    let b = append b' b'' in
-    lemma_eq_intro b' (slice b 0 (U32.v len));
+    let b'' = S.create 1 byte in
+    let b = S.append b' b'' in
+    S.lemma_eq_intro b' (S.slice b 0 (U32.v len));
     b
 
 let n_to_le_inj (len:U32.t) (n1 n2: (n:nat{n < pow2 (8 * U32.v len)})) :
@@ -126,3 +126,192 @@ let n_to_be_inj (len:U32.t) (n1 n2: (n:nat{n < pow2 (8 * U32.v len)})) :
   Lemma (requires (n_to_be len n1 == n_to_be len n2))
         (ensures (n1 == n2)) =
   ()
+
+(** A series of specializations to deal with machine integers *)
+
+let uint32_of_le (b: bytes { S.length b = 4 }) =
+  let n = le_to_n b in
+  lemma_le_to_n_is_bounded b;
+  UInt32.uint_to_t n
+
+let le_of_uint32 (x: UInt32.t): b:bytes{ S.length b = 4 } =
+  n_to_le 4ul (UInt32.v x)
+
+let uint32_of_be (b: bytes { S.length b = 4 }) =
+  let n = be_to_n b in
+  lemma_be_to_n_is_bounded b;
+  UInt32.uint_to_t n
+
+let be_of_uint32 (x: UInt32.t): b:bytes{ S.length b = 4 } =
+  n_to_be 4ul (UInt32.v x)
+
+let uint64_of_le (b: bytes { S.length b = 8 }) =
+  let n = le_to_n b in
+  lemma_le_to_n_is_bounded b;
+  UInt64.uint_to_t n
+
+let le_of_uint64 (x: UInt64.t): b:bytes{ S.length b = 8 } =
+  n_to_le 8ul (UInt64.v x)
+
+let uint64_of_be (b: bytes { S.length b = 8 }) =
+  let n = be_to_n b in
+  lemma_be_to_n_is_bounded b;
+  UInt64.uint_to_t n
+
+let be_of_uint64 (x: UInt64.t): b:bytes{ S.length b = 8 } =
+  n_to_be 8ul (UInt64.v x)
+
+let rec seq_uint32_of_le (l: nat) (b: bytes{ S.length b = 4 * l }):
+  s:S.seq UInt32.t { S.length s = l }
+=
+  if S.length b = 0 then
+    S.empty
+  else
+    let hd, tl = Seq.split b 4 in
+    S.cons (uint32_of_le hd) (seq_uint32_of_le (l - 1) tl)
+
+let rec le_of_seq_uint32 (s: S.seq UInt32.t):
+  Tot (b:bytes { S.length b = 4 * S.length s })
+    (decreases (S.length s))
+=
+  if S.length s = 0 then
+    S.empty
+  else
+    S.append (le_of_uint32 (S.head s)) (le_of_seq_uint32 (S.tail s))
+
+let rec seq_uint32_of_be (l: nat) (b: bytes{ S.length b = 4 * l }):
+  s:S.seq UInt32.t { S.length s = l }
+=
+  if S.length b = 0 then
+    S.empty
+  else
+    let hd, tl = Seq.split b 4 in
+    S.cons (uint32_of_be hd) (seq_uint32_of_be (l - 1) tl)
+
+let rec be_of_seq_uint32 (s: S.seq UInt32.t):
+  Tot (b:bytes { S.length b = 4 * S.length s })
+    (decreases (S.length s))
+=
+  if S.length s = 0 then
+    S.empty
+  else
+    S.append (be_of_uint32 (S.head s)) (be_of_seq_uint32 (S.tail s))
+
+let rec seq_uint64_of_le (l: nat) (b: bytes{ S.length b = 8 * l }):
+  s:S.seq UInt64.t { S.length s = l }
+=
+  if S.length b = 0 then
+    S.empty
+  else
+    let hd, tl = Seq.split b 8 in
+    S.cons (uint64_of_le hd) (seq_uint64_of_le (l - 1) tl)
+
+let rec le_of_seq_uint64 (s: S.seq UInt64.t):
+  Tot (b:bytes { S.length b = 8 * S.length s })
+    (decreases (S.length s))
+=
+  if S.length s = 0 then
+    S.empty
+  else
+    S.append (le_of_uint64 (S.head s)) (le_of_seq_uint64 (S.tail s))
+
+let rec seq_uint64_of_be (l: nat) (b: bytes{ S.length b = 8 * l }):
+  s:S.seq UInt64.t { S.length s = l }
+=
+  if S.length b = 0 then
+    S.empty
+  else
+    let hd, tl = Seq.split b 8 in
+    S.cons (uint64_of_be hd) (seq_uint64_of_be (l - 1) tl)
+
+let rec be_of_seq_uint64 (s: S.seq UInt64.t):
+  Tot (b:bytes { S.length b = 8 * S.length s })
+    (decreases (S.length s))
+=
+  if S.length s = 0 then
+    S.empty
+  else
+    S.append (be_of_uint64 (S.head s)) (be_of_seq_uint64 (S.tail s))
+
+
+#set-options "--max_fuel 1 --max_ifuel 0 --z3rlimit 50"
+
+let rec offset_uint32_be (b: bytes) (n: nat) (i: nat):
+  Lemma
+    (requires (
+      S.length b = 4 * n /\
+      i < n))
+    (ensures (
+      S.index (seq_uint32_of_be n b) i == uint32_of_be (S.slice b (4 * i) (4 * i + 4))))
+    (decreases (
+      S.length b))
+    [ SMTPat (S.index (seq_uint32_of_be n b) i) ]
+=
+  if S.length b = 0 then
+    false_elim ()
+  else
+    let hd, tl = Seq.split b 4 in
+    if i = 0 then
+      ()
+    else
+      offset_uint32_be tl (n - 1) (i - 1)
+
+let rec offset_uint32_le (b: bytes) (n: nat) (i: nat):
+  Lemma
+    (requires (
+      S.length b = 4 * n /\
+      i < n))
+    (ensures (
+      S.index (seq_uint32_of_le n b) i == uint32_of_le (S.slice b (4 * i) (4 * i + 4))))
+    (decreases (
+      S.length b))
+    [ SMTPat (S.index (seq_uint32_of_le n b) i) ]
+=
+  if S.length b = 0 then
+    false_elim ()
+  else
+    let hd, tl = Seq.split b 4 in
+    if i = 0 then
+      ()
+    else
+      offset_uint32_le tl (n - 1) (i - 1)
+
+let rec offset_uint64_be (b: bytes) (n: nat) (i: nat):
+  Lemma
+    (requires (
+      S.length b = 8 * n /\
+      i < n))
+    (ensures (
+      S.index (seq_uint64_of_be n b) i == uint64_of_be (S.slice b (8 * i) (8 * i + 8))))
+    (decreases (
+      S.length b))
+    [ SMTPat (S.index (seq_uint64_of_be n b) i) ]
+=
+  if S.length b = 0 then
+    false_elim ()
+  else
+    let hd, tl = Seq.split b 8 in
+    if i = 0 then
+      ()
+    else
+      offset_uint64_be tl (n - 1) (i - 1)
+
+let rec offset_uint64_le (b: bytes) (n: nat) (i: nat):
+  Lemma
+    (requires (
+      S.length b = 8 * n /\
+      i < n))
+    (ensures (
+      S.index (seq_uint64_of_le n b) i == uint64_of_le (S.slice b (8 * i) (8 * i + 8))))
+    (decreases (
+      S.length b))
+    [ SMTPat (S.index (seq_uint64_of_le n b) i) ]
+=
+  if S.length b = 0 then
+    false_elim ()
+  else
+    let hd, tl = Seq.split b 8 in
+    if i = 0 then
+      ()
+    else
+      offset_uint64_le tl (n - 1) (i - 1)
